\documentclass{article}
\usepackage[utf8]{inputenc}

\begin{document}
\maketitle

\section{Introduction}
\\2.1
\\While j = 1, 
\begin{equation*}
\\v_j(y_j) = max_{{y_{j-1}}} s(x,j,y_{j-1},y_j)
\end{equation*}
    \\Assume that for all j, 
\begin{equation*}
\\v_j(y_j) = max_{{y_{j-1}}} [s(x,j,y_{j-1},y_j) + v_{j-1}(y_{j-1})]
\end{equation*}
\\We want prove that for 
\begin{equation*}
{j+1}, \\v_{j+1}(y_{j+1}) = max_{{y_{j}}} [s(x,j,y_{j},y_{j+1}) + v_{j}(y_{j})]
\end{equation*}
\\
\begin{equation*}
\\v_{j+1}(y_{j+1}) = max_{{y_1},..,{y_{j}}}\sum_{i=1}^{j+1}s(x,j,y_{j-1},y_j)
= max_{{y_{j}}} [s(x,j,y_{j},y_{j+1}) + max_{{y_{j-1}}} [s(x,j,y_{j-1},y_j) + max_{{y_{j-2}}}......)]] = max_{{y_{j}}} [s(x,j,y_{j},y_{j+1}) + v_{j}(y_{j})]
\end{equation*}
\\
\\2.2
\begin{equation*}
\\O(K^2N) 
\end{equation*}
\\where K is the number of state, N is the length of the sequence


\end{document}
